configure.sh
@@ -1,3 +1,4 @@
 #!/usr/bin/env bash
 opam repo add coq-released https://coq.inria.fr/opam/released
-opam install coq-relation-algebra
+opam repo add coq-released-hahn https://github.com/vafeiadis/hahn.git
+opam install coq-relation-algebra coq-hahn
